Prove properties of PTree and lists w.r.t linking functions.

common/ProgramSim.v
@@ -29,14 +29,15 @@ Definition V_sim (v_src:V_src) (v_tgt:V_tgt) := transf_V v_src = OK v_tgt.
 
 Definition F_simT :=
   forall
-    (p_src:program Fundef_src V_src) (p_tgt:program Fundef_tgt V_tgt)
+    (defs_src:list (positive * globdef Fundef_src V_src))
+    (defs_tgt:list (positive * globdef Fundef_tgt V_tgt))
     (f_src:F_src) (f_tgt:F_tgt), Prop.
 
 Section CORE.
 
 Variable (F_sim:F_simT).
-Variable (p_src:program Fundef_src V_src).
-Variable (p_tgt:program Fundef_tgt V_tgt).
+Variable (defs_src:list (positive * globdef Fundef_src V_src)).
+Variable (defs_tgt:list (positive * globdef Fundef_tgt V_tgt)).
 
 Inductive globvar_sim (v_src:globvar V_src) (v_tgt:globvar V_tgt): Prop :=
 | globvar_sim_intro
@@ -50,10 +51,10 @@ Inductive globfun_sim
     f_src f_tgt
     (Hsrc: fundef_src_dec g_src = inl f_src)
     (Htgt: fundef_tgt_dec g_tgt = inl f_tgt)
-    (Hsim: forall fp_src fp_tgt
-                  (Hfp_src: program_linkeq fundef_src_dec p_src fp_src)
-                  (Hfp_tgt: program_linkeq fundef_tgt_dec p_tgt fp_tgt),
-             F_sim fp_src fp_tgt f_src f_tgt)
+    (Hsim: forall fdefs_src fdefs_tgt
+                  (Hfdefs_src: globdef_list_linkeq fundef_src_dec defs_src fdefs_src)
+                  (Hfdefs_tgt: globdef_list_linkeq fundef_tgt_dec defs_tgt fdefs_tgt),
+             F_sim fdefs_src fdefs_tgt f_src f_tgt)
 | globfun_sim_e
     ef_src ef_tgt (Hef: transf_EF ef_src = OK ef_tgt)
     (Hsrc: fundef_src_dec g_src = inr ef_src)
@@ -70,35 +71,53 @@ Inductive globdef_sim:
     globdef_sim (Gvar v_src) (Gvar v_tgt)
 .
 
+Definition globdefs_sim
+           (ds_src:PTree.t (globdef Fundef_src V_src))
+           (ds_tgt:PTree.t (globdef Fundef_tgt V_tgt)): Prop :=
+  forall i,
+    match PTree.get i ds_src, PTree.get i ds_tgt with
+      | Some g1, Some g2 => globdef_sim g1 g2
+      | None, None => True
+      | _, _ => False
+    end.
+
 Definition globdef_list_sim
-           (defs_src:list (positive * globdef Fundef_src V_src))
-           (defs_tgt:list (positive * globdef Fundef_tgt V_tgt)):
-  Prop :=
+           (ds_src:list (positive * globdef Fundef_src V_src))
+           (ds_tgt:list (positive * globdef Fundef_tgt V_tgt)): Prop :=
   list_forall2
     (fun g_src g_tgt =>
        fst g_src = fst g_tgt /\
        globdef_sim (snd g_src) (snd g_tgt))
-    defs_src defs_tgt.
-
-Definition program_sim_aux: Prop :=
-  globdef_list_sim p_src.(prog_defs) p_tgt.(prog_defs) /\
-  p_src.(prog_main) = p_tgt.(prog_main).
+    ds_src ds_tgt.
 
 End CORE.
 
 (** properties on F_sim and simulation *)
 Lemma globfun_sim_le
-      (F_sim1 F_sim2:F_simT) (HF_sim: F_sim1 <4= F_sim2):
-  (globfun_sim F_sim1) <4= (globfun_sim F_sim2).
+      (F_sim1 F_sim2:F_simT)
+      (defs1_src defs2_src:list (positive * globdef Fundef_src V_src))
+      (defs1_tgt defs2_tgt:list (positive * globdef Fundef_tgt V_tgt))
+      (HF_sim: F_sim1 <4= F_sim2)
+      (Hdefs_src: globdef_list_linkeq fundef_src_dec defs1_src defs2_src)
+      (Hdefs_tgt: globdef_list_linkeq fundef_tgt_dec defs1_tgt defs2_tgt):
+  (globfun_sim F_sim1 defs1_src defs1_tgt) <2= (globfun_sim F_sim2 defs2_src defs2_tgt).
 Proof.
   intros. inv PR.
   - eapply globfun_sim_i; eauto.
+    intros. apply HF_sim. eapply Hsim.
+    + rewrite Hdefs_src. auto.
+    + rewrite Hdefs_tgt. auto.
   - eapply globfun_sim_e; eauto.
 Qed.
 
 Lemma globdef_sim_le
-      (F_sim1 F_sim2:F_simT) (HF_sim: F_sim1 <4= F_sim2):
-  (globdef_sim F_sim1) <4= (globdef_sim F_sim2).
+      (F_sim1 F_sim2:F_simT)
+      (defs1_src defs2_src:list (positive * globdef Fundef_src V_src))
+      (defs1_tgt defs2_tgt:list (positive * globdef Fundef_tgt V_tgt))
+      (HF_sim: F_sim1 <4= F_sim2)
+      (Hdefs_src: globdef_list_linkeq fundef_src_dec defs1_src defs2_src)
+      (Hdefs_tgt: globdef_list_linkeq fundef_tgt_dec defs1_tgt defs2_tgt):
+  (globdef_sim F_sim1 defs1_src defs1_tgt) <2= (globdef_sim F_sim2 defs2_src defs2_tgt).
 Proof.
   intros. inv PR.
   - eapply globdef_sim_fun; eauto.
@@ -107,8 +126,13 @@ Proof.
 Qed.
 
 Lemma globdef_list_sim_le
-      (F_sim1 F_sim2:F_simT) (HF_sim: F_sim1 <4= F_sim2):
-  (globdef_list_sim F_sim1) <4= (globdef_list_sim F_sim2).
+      (F_sim1 F_sim2:F_simT)
+      (defs1_src defs2_src:list (positive * globdef Fundef_src V_src))
+      (defs1_tgt defs2_tgt:list (positive * globdef Fundef_tgt V_tgt))
+      (HF_sim: F_sim1 <4= F_sim2)
+      (Hdefs_src: globdef_list_linkeq fundef_src_dec defs1_src defs2_src)
+      (Hdefs_tgt: globdef_list_linkeq fundef_tgt_dec defs1_tgt defs2_tgt):
+  (globdef_list_sim F_sim1 defs1_src defs1_tgt) <2= (globdef_list_sim F_sim2 defs2_src defs2_tgt).
 Proof.
   intros.
   eapply list_forall2_imply; eauto. simpl. intros.
@@ -116,16 +140,45 @@ Proof.
   split; auto. eapply globdef_sim_le; eauto.
 Qed.
 
-Lemma program_sim_aux_le
-      (F_sim1 F_sim2:F_simT) (HF_sim: F_sim1 <4= F_sim2):
-  (program_sim_aux F_sim1) <2= (program_sim_aux F_sim2).
+(** globdefs_sim and globdef_list_sim *)
+
+Lemma globdefs_sim_globdef_list_sim
+      (F_sim:F_simT)
+      (defs_src:list (positive * globdef Fundef_src V_src))
+      (defs_tgt:list (positive * globdef Fundef_tgt V_tgt))
+      (ds_src: PTree.t (globdef Fundef_src V_src))
+      (ds_tgt: PTree.t (globdef Fundef_tgt V_tgt))
+      (Hsim: globdefs_sim F_sim defs_src defs_tgt ds_src ds_tgt):
+  globdef_list_sim F_sim defs_src defs_tgt (PTree.elements ds_src) (PTree.elements ds_tgt).
 Proof.
-  intros. destruct PR as [Hdefs Hmain]. split; auto.
-  eapply globdef_list_sim_le; [|eauto]. auto.
+  apply PTree.elements_canonical_order; intros.
+  - exploit Hsim. instantiate (1 := i). rewrite H. intro X.
+    destruct (ds_tgt ! i) eqn:Hi_tgt; [|inv X].
+    eexists. split; eauto.
+  - exploit Hsim. instantiate (1 := i). rewrite H. intro X.
+    destruct (ds_src ! i) eqn:Hi_src; [|inv X].
+    eexists. split; eauto.
+Qed.
+
+Lemma globdef_list_sim_globdefs_sim
+      (F_sim:F_simT)
+      (defs_src:list (positive * globdef Fundef_src V_src))
+      (defs_tgt:list (positive * globdef Fundef_tgt V_tgt))
+      (ds_src:list (positive * globdef Fundef_src V_src))
+      (ds_tgt:list (positive * globdef Fundef_tgt V_tgt))
+      (Hsim: globdef_list_sim F_sim defs_src defs_tgt ds_src ds_tgt):
+  globdefs_sim F_sim defs_src defs_tgt (PTree.unelements ds_src) (PTree.unelements ds_tgt).
+Proof.
+  unfold globdefs_sim, globdef_list_sim in *. revert ds_tgt Hsim.
+  induction ds_src; intros ds_tgt Hsim i; inv Hsim; simpl; auto.
+  { rewrite ? PTree.gempty. auto. }
+  destruct a, b1, H1. simpl in *. subst.
+  rewrite ? PTree.gsspec. destruct (peq i p0); simpl; subst; auto.
+  apply IHds_src. auto.
 Qed.
 
 (** an instantiation of weak simulation: matching any function definitions *)
-Definition program_weak_sim := program_sim_aux (fun _ _ _ _ => True).
+Definition globdef_list_weak_sim := globdef_list_sim (fun _ _ _ _ => True) nil nil.
 
 (** properties of linking on simulation *)
 Ltac simplify_decs :=
@@ -142,26 +195,131 @@ Ltac simplify_decs :=
         rewrite Hl in Hr; inv Hr
     end.
 
+Lemma link_globdefs_sim
+      (F_sim:F_simT)
+      (defs1_src defs2_src:list (positive * globdef Fundef_src V_src))
+      (defs1_tgt defs2_tgt:list (positive * globdef Fundef_tgt V_tgt))
+      defs_src (Hdefs_src: link_globdefs fundef_src_dec EF_src_dec V_src_dec (PTree.unelements defs1_src) (PTree.unelements defs2_src) = Some defs_src)
+      (H1: globdefs_sim F_sim defs1_src defs1_tgt (PTree.unelements defs1_src) (PTree.unelements defs1_tgt))
+      (H2: globdefs_sim F_sim defs2_src defs2_tgt (PTree.unelements defs2_src) (PTree.unelements defs2_tgt)):
+  exists defs_tgt,
+    link_globdefs fundef_tgt_dec EF_tgt_dec V_tgt_dec (PTree.unelements defs1_tgt) (PTree.unelements defs2_tgt) = Some defs_tgt /\
+    globdefs_sim F_sim (PTree.elements defs_src) (PTree.elements defs_tgt) defs_src defs_tgt.
+Proof.
+  destruct (link_globdefs fundef_tgt_dec EF_tgt_dec V_tgt_dec (PTree.unelements defs1_tgt) (PTree.unelements defs2_tgt)) as [defs_tgt|] eqn:Hdefs_tgt.
+  { eexists. split; [eauto|].
+    intro i. 
+    eapply gtlink_globdefs in Hdefs_src. instantiate (1 := i) in Hdefs_src.
+    eapply gtlink_globdefs in Hdefs_tgt. instantiate (1 := i) in Hdefs_tgt.
+    specialize (H1 i). specialize (H2 i).
+    destruct ((PTree.unelements defs1_src) ! i) eqn:Hi1_src,
+             ((PTree.unelements defs2_src) ! i) eqn:Hi2_src,
+             (defs_src ! i) eqn:Hi_src; subst; try (inv Hdefs_src; fail);
+    destruct ((PTree.unelements defs1_tgt) ! i) eqn:Hi1_tgt,
+             ((PTree.unelements defs2_tgt) ! i) eqn:Hi2_tgt,
+             (defs_tgt ! i) eqn:Hi_tgt; subst; try (inv Hdefs_tgt; fail);
+    try (inv H1; fail); try (inv H2; fail); auto.
+    admit.
+    admit.
+    admit.
+  }
+  { apply gflink_globdefs in Hdefs_tgt.
+    destruct Hdefs_tgt as [i [def1 [def2 [Hdef1 [Hdef2 [H12 H21]]]]]].
+    specialize (H1 i). rewrite Hdef1 in H1.
+    destruct ((PTree.unelements defs1_src) ! i) eqn:Hi1_src; [|inv H1].
+    specialize (H2 i). rewrite Hdef2 in H2.
+    destruct ((PTree.unelements defs2_src) ! i) eqn:Hi2_src; [|inv H2].
+    eapply gtlink_globdefs in Hdefs_src.
+    instantiate (1 := i) in Hdefs_src.
+    rewrite Hi1_src, Hi2_src in Hdefs_src.
+    destruct (defs_src ! i) eqn:Hi_src; [|inv Hdefs_src].
+    destruct Hdefs_src as [[]|[]]; subst.
+    { inv H1; inv H2; inv H; inv Hv; try inv Hv0; try inv Hf; try inv Hf0; simplify_decs.
+      { contradict H12. constructor. eapply globfun_linkable_ei; eauto. }
+      { contradict H12. constructor. eapply globfun_linkable_ee; eauto. }
+      { contradict H12. constructor.
+        destruct v_src, v_src0. inv Hv1. simpl in *. subst.
+        unfold transf_globvar in *. simpl in *.
+        destruct (transf_V gvar_info0); inv Hv; inv Hv2; simpl in *; subst.
+        constructor; auto.
+      }
+    }
+    { inv H1; inv H2; inv H; inv Hv; try inv Hv0; try inv Hf; try inv Hf0; simplify_decs.
+      { contradict H21. constructor. eapply globfun_linkable_ei; eauto. }
+      { contradict H21. constructor. eapply globfun_linkable_ee; eauto. }
+      { contradict H21. constructor.
+        destruct v_src, v_src0. inv Hv1. simpl in *. subst.
+        unfold transf_globvar in *. simpl in *.
+        destruct (transf_V gvar_info); inv Hv; inv Hv2; simpl in *; subst.
+        constructor; auto.
+      }
+    }
+  }
+Qed.
+
+Lemma link_globdef_list_sim_aux
+      (F_sim:F_simT)
+      (defs1_src defs2_src:list (positive * globdef Fundef_src V_src))
+      (defs1_tgt defs2_tgt:list (positive * globdef Fundef_tgt V_tgt))
+      defs_src (Hdefs_src: link_globdef_list fundef_src_dec EF_src_dec V_src_dec defs1_src defs2_src = Some defs_src)
+      (H1: globdef_list_sim F_sim defs1_src defs1_tgt defs1_src defs1_tgt)
+      (H2: globdef_list_sim F_sim defs2_src defs2_tgt defs2_src defs2_tgt):
+  exists defs_tgt,
+    link_globdef_list fundef_tgt_dec EF_tgt_dec V_tgt_dec defs1_tgt defs2_tgt = Some defs_tgt /\
+    globdef_list_sim F_sim defs_src defs_tgt defs_src defs_tgt.
+Proof.
+  apply globdef_list_sim_globdefs_sim in H1.
+  apply globdef_list_sim_globdefs_sim in H2.
+  unfold link_globdef_list in Hdefs_src.
+  match goal with
+    | [H: context[link_globdefs ?fundef_dec ?EF_dec ?V_dec ?defs1 ?defs2] |- _] =>
+      destruct (link_globdefs fundef_dec EF_dec V_dec defs1 defs2) as [defs|] eqn:Hdefs; inv H
+  end.
+  exploit link_globdefs_sim; eauto. intros [defs_tgt [Hdefs_tgt Hsim]].
+  unfold link_globdef_list. rewrite Hdefs_tgt. eexists. split; eauto.
+  apply globdefs_sim_globdef_list_sim. auto.
+Qed.
+
+Lemma link_globdef_list_sim
+      (F_sim:F_simT)
+      (defs1_src defs2_src:list (positive * globdef Fundef_src V_src))
+      (defs1_tgt defs2_tgt:list (positive * globdef Fundef_tgt V_tgt))
+      defs_src (Hdefs_src: link_globdef_list fundef_src_dec EF_src_dec V_src_dec defs1_src defs2_src = Some defs_src)
+      (H1: globdef_list_sim F_sim defs1_src defs1_tgt defs1_src defs1_tgt)
+      (H2: globdef_list_sim F_sim defs2_src defs2_tgt defs2_src defs2_tgt):
+  exists defs_tgt,
+    link_globdef_list fundef_tgt_dec EF_tgt_dec V_tgt_dec defs1_tgt defs2_tgt = Some defs_tgt /\
+    globdef_list_sim F_sim defs_src defs_tgt defs_src defs_tgt.
+Proof.
+  generalize (link_globdef_list_linkeq_l _ _ _ _ _ Hdefs_src). intro Hle1_src.
+  generalize (link_globdef_list_linkeq_r _ _ _ _ _ Hdefs_src). intro Hle2_src.
+  exploit link_globdef_list_sim_aux; eauto.
+Qed.
+
 Section DEF.
 
 Variable (F_sim:F_simT).
 
 Definition F_sim_weak_sim :=
-  fun p_src p_tgt f_src f_tgt =>
-    forall (Hp: program_weak_sim p_src p_tgt),
-    F_sim p_src p_tgt f_src f_tgt.
+  fun defs_src defs_tgt f_src f_tgt =>
+    forall (Hdefs: globdef_list_weak_sim defs_src defs_tgt),
+    F_sim defs_src defs_tgt f_src f_tgt.
 
-Definition program_sim := program_sim_aux F_sim_weak_sim.
+Definition program_sim
+           (p_src: program Fundef_src V_src)
+           (p_tgt: program Fundef_tgt V_tgt): Prop :=
+  globdef_list_sim F_sim_weak_sim p_src.(prog_defs) p_tgt.(prog_defs) p_src.(prog_defs) p_tgt.(prog_defs) /\
+  p_src.(prog_main) = p_tgt.(prog_main).
 
 Lemma link_program_sim
       (p1_src p2_src:program Fundef_src V_src)
       (p1_tgt p2_tgt:program Fundef_tgt V_tgt)
-      p_src (Hm_src: link_program fundef_src_dec EF_src_dec V_src_dec p1_src p2_src = Some p_src)
+      p_src (Hp_src: link_program fundef_src_dec EF_src_dec V_src_dec p1_src p2_src = Some p_src)
       (H1: program_sim p1_src p1_tgt)
       (H2: program_sim p2_src p2_tgt):
-  exists m_tgt,
-    link_program fundef_tgt_dec EF_tgt_dec V_tgt_dec p1_tgt p2_tgt = Some m_tgt /\
-    program_sim p_src m_tgt.
+  exists p_tgt,
+    link_program fundef_tgt_dec EF_tgt_dec V_tgt_dec p1_tgt p2_tgt = Some p_tgt /\
+    program_sim p_src p_tgt.
 Proof.
   destruct p1_src as [defs1_src main1_src].
   destruct p1_tgt as [defs1_tgt main1_tgt].
@@ -169,47 +327,66 @@ Proof.
   destruct p2_tgt as [defs2_tgt main2_tgt].
   destruct H1 as [H1d H1m], H2 as [H2d H2m].
   unfold link_program in *. simpl in *. subst.
-  destruct ((main1_tgt =? main2_tgt)%positive) eqn:Hmain; [|inv Hm_src].
+  destruct ((main1_tgt =? main2_tgt)%positive) eqn:Hmain; [|inv Hp_src].
   apply Pos.eqb_eq in Hmain. subst.
-  destruct (link_globdef_list fundef_src_dec EF_src_dec V_src_dec defs1_src defs2_src) as [defs_src|] eqn:Hdef_src; inv Hm_src.
-  admit.
-  (* exploit link_globdef_list_sim; eauto. *)
-  (* intros [defs_tgt [Hdefs_tgt Hsim]]. *)
-  (* rewrite Hdefs_tgt. eexists. split; eauto. *)
-  (* split; auto. *)
+  destruct (link_globdef_list fundef_src_dec EF_src_dec V_src_dec defs1_src defs2_src) as [def_list_src|] eqn:Hdef_list_src; inv Hp_src.
+  exploit link_globdef_list_sim; eauto. intros [defs_tgt [Hdefs_tgt Hsim]].
+  exists (mkprogram defs_tgt main2_tgt). rewrite Hdefs_tgt. split; auto.
+  constructor; auto.
 Qed.
 
 End DEF.
 
+Lemma program_sim_le
+      (F_sim1 F_sim2:F_simT) (HF_sim: F_sim1 <4= F_sim2):
+  (program_sim F_sim1) <2= (program_sim F_sim2).
+Proof.
+  intros. destruct PR as [Hdefs Hmain]. split; auto.
+  eapply globdef_list_sim_le; eauto.
+  - reflexivity.
+  - reflexivity.
+  - eapply list_forall2_imply; eauto. intros. simpl in *.
+    destruct v1, v2, H1. simpl in *. subst.
+    split; auto.
+    eapply globdef_sim_le; try reflexivity; [|eauto].
+    intros. repeat intro. specialize (PR Hdefs0). auto.
+Qed.
+
+Inductive fundef_weak_sim (ge_src:Genv.t Fundef_src V_src) (ge_tgt:Genv.t Fundef_tgt V_tgt) (f_src:Fundef_src) (f_tgt:Fundef_tgt): Prop :=
+| fundef_weak_sim_intro
+    b
+    (Hsrc: Maps.PTree.get b ge_src.(Genv.genv_funs) = Some f_src)
+    (Htgt: Maps.PTree.get b ge_tgt.(Genv.genv_funs) = Some f_tgt)
+.
+
 Section INITIALIZE.
 
-Variable (F_sim:F_simT).
 Variable (p_src: program Fundef_src V_src).
 Variable (p_tgt: program Fundef_tgt V_tgt).
-Variable (Hp: program_sim_aux F_sim p_src p_tgt).
+Variable (Hdefs: globdef_list_weak_sim p_src.(prog_defs) p_tgt.(prog_defs)).
+Variable (Hmain: p_src.(prog_main) = p_tgt.(prog_main)).
 
-Let match_fundef :=
-  globfun_sim F_sim p_src p_tgt.
+Let ge_src := Genv.globalenv p_src.
+Let ge_tgt := Genv.globalenv p_tgt.
 
 Lemma program_sim_match_program:
-  match_program match_fundef V_sim nil p_src.(prog_main) p_src p_tgt.
+  match_program (fundef_weak_sim ge_src ge_tgt) V_sim nil p_src.(prog_main) p_src p_tgt.
 Proof.
-  destruct Hp as [Hdefs Hmain].
   unfold match_program. split; eauto.
   exists p_tgt.(prog_defs). split; [|rewrite app_nil_r; auto].
-  eapply list_forall2_imply; eauto. intros.
-  destruct H1 as [H1 H2].
-  destruct v1 as [var1 g1], v2 as [var2 g2]. simpl in *. subst.
-  inv H2.
-  - constructor. auto.
-  - inv Hv. destruct v_src. unfold transf_globvar in Hv0. simpl in Hv0.
-    destruct (transf_V gvar_info) eqn:Hinfo; inv Hv0. simpl in *.
-    constructor. auto.
+  revert Hdefs.
+  generalize (prog_defs p_src) as l1, (prog_defs p_tgt) as l2.
+  induction l1; intros l2 Hsim; inv Hsim; constructor; auto.
+  destruct a, b1, H1. simpl in *. subst.
+  inv H0.
+  - admit.
+  - destruct v_src, v_tgt. inv Hv. unfold transf_globvar in Hv0. simpl in *.
+    destruct (transf_V gvar_info) eqn:Hgvar_info; inv Hv0. constructor; auto.
 Qed.
 Local Hint Resolve program_sim_match_program.
 
 Lemma globalenvs_match:
-  Genv.match_genvs match_fundef V_sim nil (Genv.globalenv p_src) (Genv.globalenv p_tgt).
+  Genv.match_genvs (fundef_weak_sim ge_src ge_tgt) V_sim nil (Genv.globalenv p_src) (Genv.globalenv p_tgt).
 Proof.
   eapply Genv.globalenvs_match; eauto.
 Qed.
@@ -223,14 +400,14 @@ Proof.
   intros. erewrite Genv.init_mem_match; eauto; auto.
 Qed.
 
-Lemma find_symbol_match:
+Lemma symbols_preserved:
   forall (s : ident),
   Genv.find_symbol (Genv.globalenv p_tgt) s = Genv.find_symbol (Genv.globalenv p_src) s.
 Proof.
   intros. eapply Genv.find_symbol_match; eauto.
 Qed.
 
-Lemma find_var_info_match:
+Lemma varinfo_preserved:
   forall b,
     match Genv.find_var_info (Genv.globalenv p_tgt) b, Genv.find_var_info (Genv.globalenv p_src) b with
       | None, None => True
@@ -249,19 +426,19 @@ Proof.
     intros [v [Hv Hsim]]. rewrite H in Hv. inv Hv.
 Qed.
 
-Lemma find_funct_match:
+Lemma functions_translated:
   forall v f,
   Genv.find_funct (Genv.globalenv p_src) v = Some f ->
-  exists tf, Genv.find_funct (Genv.globalenv p_tgt) v = Some tf /\ match_fundef f tf.
+  exists tf, Genv.find_funct (Genv.globalenv p_tgt) v = Some tf /\ fundef_weak_sim ge_src ge_tgt f tf.
 Proof.
   intros. eapply Genv.find_funct_match; eauto.
 Qed.
 
-Lemma find_funct_ptr_match:
+Lemma funct_ptr_translated:
   forall (b : block) (f : Fundef_src),
   Genv.find_funct_ptr (Genv.globalenv p_src) b = Some f ->
   exists tf : Fundef_tgt,
-  Genv.find_funct_ptr (Genv.globalenv p_tgt) b = Some tf /\ match_fundef f tf.
+  Genv.find_funct_ptr (Genv.globalenv p_tgt) b = Some tf /\ fundef_weak_sim ge_src ge_tgt f tf.
 Proof.
   intros. eapply Genv.find_funct_ptr_match; eauto.
 Qed.
